First version of updated proof of merge.

coq-osiris/examples/proofs/merge.v
@@ -5,24 +5,6 @@ From osiris.stdlib Require Import Stdlib.
 From osiris.logic Require Import sorting.
 From osiris.examples Require Import og_merge.
 
-
-Notation "'Environment'  'composed'  'of'  [ x ; .. ; z ]" :=
-  (cons x _ (.. (cons z _ nil) ..))
- (only printing).
-
-(* TODO Move *)
-(* [call_spec] is the type of specifications over function calls. It
-   depends on two arguments: the argument of the function call, and the
-   computation resulting from the function call on that argument. *)
-
-Definition call_spec {X : Type} := X -> microvx -> Prop.
-
-(* [Spec c P] states that given a closure [c], the specification [P]
-   holds for a call of [c] on any argument. *)
-
-Definition Spec `{Encode X} (c : val) (P : call_spec) :=
-  ∀ (arg : X), P arg (call c #arg).
-
 (* -------------------------------------------------------------------------- *)
 
 (* WIP: Tactics used in local proof scripts. *)
@@ -124,17 +106,13 @@ Next Obligation. intros. apply wf_inverse_image, lt_wf. Qed.
 
 (* Specification for [merge l1 l2]. *)
 
-Local Definition merge_pre :=
-  (fun l1 l2 => Forall representable l1 /\ Forall representable l2
-             /\ Sorted Z.le l1 /\ Sorted Z.le l2).
-Local Definition merge_post := (fun l1 l2 l => Sorted Z.le l /\ Permutation (l1++l2) l).
-Local Hint Unfold merge_post : core.
-Local Hint Unfold merge_pre : core.
+Definition merge_spec (l1 : list Z) (l2 : list Z) (m : microvx) : Prop :=
+  (* Preconditions on [l1] and [l2]. *)
+  Forall representable l1 ∧ Sorted Z.le l1 ->
+  Forall representable l2 ∧ Sorted Z.le l2 ->
+  (* Specification of the function call [merge l1 l2]. *)
+  pure m (λ l, Sorted Z.le l ∧ Permutation (l1++l2) l) ⊥.
 
-Definition merge_spec (merge : val) : Prop :=
-  ∀ (l1 l2 : list Z),
-    merge_pre l1 l2 ->
-    pure_call2 merge #l1 #l2 (merge_post l1 l2) ⊥.
 
 (* Specification for [split l]. *)
 
@@ -144,12 +122,17 @@ Local Definition split_post {A} :=
             else length p.1 = S (Nat.div2 (length l)))
            /\ length p.2 = Nat.div2 (length l) /\ Permutation (p.1 ++ p.2) l).
 
-Definition split_spec (split : val) : Prop :=
-  ∀ A `(_ : Encode A) (l : list A),
-    pure
-      (call split #l)
-      (split_post l) ⊥.
+Definition split_spec `{Encode A} (l : list A) (m : microvx) : Prop :=
+  pure m (split_post l) ⊥.
 
+
+(* Specification for [mergesort l]. *)
+
+Definition mergesort_spec (l : list Z) (m : microvx) : Prop :=
+  (* Precondition on [l]. *)
+  Forall representable l ->
+  (* Specification of the function call [mergesort l]. *)
+  pure m (λ l', Sorted Z.le l' ∧ Permutation l' l) ⊥.
 
 (* Specification for [mergesort l]. *)
 
@@ -168,14 +151,6 @@ Definition mergesort_spec' (l : list Z) (e : microvx) : Prop :=
 
 Local Ltac trivial_pure := repeat (first [ pure_path | pure_data | pure_const]).
 
-Local Ltac pure_eval_app2_conseq :=
-  eapply pure_eval_app2_conseq;
-  [ trivial_pure; reflexivity
-  | trivial_pure; reflexivity
-  | trivial_pure; reflexivity
-  |
-  | ].
-
 Local Ltac pure_EOpLe :=
   eapply pure_eval_EOpLe;
   [ trivial_pure; reflexivity
@@ -183,216 +158,277 @@ Local Ltac pure_EOpLe :=
   |
   | ].
 
-Lemma Merge_spec' η:
-  merge_spec (VCloRec η __bindings4 "merge" ).
-Proof. Admitted.
-
-Lemma Split_spec' η :
-  split_spec (VCloRec η __bindings7 "split").
-Proof.
-  unfold split_spec. intros.
-
-  eapply pure_rec_call with (P := fun _ => True); first done.
-  clear l.
-  intros split ? IH _.
-
-  (* pure_rec l (@wf_list_length A). *)
-  (* Goal: eval match on l *)
-  eapply pure_eval_match. { pure_path. }
-  pure_match.
-
-  (* First branch of match *)
-  { (* Case: l matches [] *)
-    apply pure_eval_pair. trivial_pure.
-    (* Establish the (trivial) postcondition *)
-    (* FIXME : Remove [Unshelve.] *)
-    Unshelve. 4-5: exact nil.
-    all: auto.
-    split; simpl; auto. }
-  (* Second branch of match *)
-  { (* Case: l matches [x] *)
-    apply pure_eval_pair. trivial_pure.
-    (* Establish postcondition *)
-    Unshelve. 5: exact nil. 4: exact [x0].
-    all: auto.
-    split; simpl; auto. }
-  (* Third branch of match *)
-  { (* Case: l matches a::b::t *)
-    eapply pure_eval_let_pair.
-    eapply pure_eval_app. pure_path. pure_path.
-    encode.
-    (* Call vf #xs *)
-    eapply pure_mono.
-    { (* Use induction hypothesis *)
-      apply IH.
-      { (* Justify use of induction hypothesis *)
-        simpl.
-        eauto with arith. }
-      { (* Show the precondition. *)
-        reflexivity. } }
-    intros [l1 l2] Hpost; clear IH; simpl.
-    simpl_extend; simpl. fold eval. abstract_env.
-    (* Eval (x1::l1, x2::l2) *)
-    unfold split_post in *; simpl in *.
-    destruct Hpost as (Hlength1 & Hlength2 & ?).
-    subst.
-
-    apply pure_eval_pair. trivial_pure.
-    (* Establish postcondition *)
-    Unshelve. (* FIXME : Remove [Unshelve]. *)
-    4 : exact (x :: l1). 4 : exact (x0 :: l2).
-    { cbn. unfold VCons. repeat f_equiv. }
-    { cbn. unfold VCons. repeat f_equiv. }
-    cbn. unfold VCons. repeat f_equiv.
-    split; [ | split ].
-    { (* Subgoal: the length of l1 is half the length of xs *)
-      destruct (Nat.even _); rewrite Hlength1; eauto with arith. }
-    { (* Subgoal: the length of l2 is half the length of xs *)
-      rewrite Hlength2; eauto with arith. }
-    { (* Subgoal: l1++l2 is a permutation of xs *)
-      rewrite_permutation xs'0.
-      apply Permutation_skip.
-      apply Permutation_sym.
-      apply Permutation_middle. } }
-Qed.
-
 Section merge.
 
 Variable η : env.
 
 Variable split : val.
-Hypothesis _split_spec : split_spec split.
+Hypothesis _split_spec : @Spec tele[list Z] split split_spec.
 Hypothesis Hsplit : lookup_name η "split" = ret split.
 
 Variable merge : val.
-Hypothesis _merge_spec : merge_spec merge.
+Hypothesis _merge_spec : @Spec tele[list Z; list Z] merge merge_spec.
 Hypothesis Hmerge : lookup_name η "merge" = ret merge.
 
-Lemma mergesort_mkspec mergesort l :
+Opaque Spec.
+
+Lemma mergesort_mkspec mergesort (l : list Z) :
   (lookup_name η "l" = ret #l) ->
   (lookup_name η "merge_sort" = ret mergesort) ->
-  Spec mergesort (λ l' m, length l' < length l -> mergesort_spec' l' m) ->
-  mergesort_spec' l (eval η (EMatch (EPath ["l"]) __branches11)).
-Proof. Admitted.
-
-End merge.
-
-Definition mergesort_spec (mergesort : val) : Prop :=
-  ∀ (l : list Z),
-    mergesort_pre l ->
-    pure
-      (call mergesort #l)
-      (mergesort_post l) ⊥.
-
-
-Lemma MergeSort_spec η:
-  (exists split, lookup_name η "split" = ret split /\ split_spec split) ->
-  (exists merge, lookup_name η "merge" = ret merge /\ merge_spec merge) ->
-  mergesort_spec (VCloRec η __bindings12 "merge_sort").
+  (Spec mergesort (@arg_bind _ tele[list Z] (λ x m,
+       (length x < length l)%nat ->
+       mergesort_spec x m))) ->
+  mergesort_spec l (eval η (EMatch (EPath ["l"]) __branches11)).
 Proof.
-  (* Destruct the hypotheses on split and merge *)
-  destruct 1 as (split&Hsplit&_split_spec).
-  destruct 1 as (merge&Hmerge&_merge_spec).
-  unfold mergesort_spec; intros l ?.
-  eapply pure_rec_call with (P := mergesort_pre).
-  { assumption. }
-  clear H l.
-  intros mergesort l IH Hpre.
+  intros Hl Hmergesort IH Hpre.
 
-  eapply pure_eval_match. { pure_path. }
-  pure_match; abstract_env.
-  { pure_const. auto. } (* Branch: "[]"  *)
-  { pure_data. auto. }  (* Branch: "[x]" *)
+  eapply pure_eval_match. { eapply pure_eval_path.
+                            simpl. rewrite Hl. pure_ret. }
+  pure_match.
+  (* Branch: "[]"  *)
+  { pure_const. auto. }
+  (* Branch: "[x]" *)
+  { eapply pure_eval_data. eapply pure_evals_cons.
+    pure_path. simpl; encode.
+    eapply pure_evals_cons. eapply pure_eval_const with (x := @nil Z).
+    encode.
+    eapply pure_evals_nil. exists [x]. split; [ encode | auto ]. }
 
   (* Branch: "_" *)
   { assert (exists m, length (x0) = S m) as [m Heql].
     { subst. destruct x0; [ congruence | eauto ]. }
+    simpl in IH. rewrite Heql in IH.
     eapply pure_eval_let_pair.
-    eapply pure_eval_app.
-    (* Use knowledge that [split] ∈ [η] *)
-    eapply pure_eval_path. simpl. rewrite Hsplit.
-    pure_ret.
-    pure_path.
-    (* FIXME Remove *) Unshelve. 8 : exact (x :: x0).
-    encode. 2-5:shelve.
-
     (* Use knowledge that [split] ⊨ [split_spec] *)
-    eapply pure_mono. { apply _split_spec. }
-    intros [l1 l2] (Hl1 & Hl2 & Hperm); simpl in *.
-    unfold mergesort_pre in Hpre;
-      rewrite <- Hperm in Hpre; apply Forall_app in Hpre as [??].
+    eapply (pure_EApp tele[list Z]).
+    { eapply pure_eval_path. simpl. rewrite Hsplit.
+      pure_ret. }
+    { eapply pure_eval_path. simpl. rewrite Hl.
+      eapply pure_ret. encode. apply eq_refl. }
+    unfold arg_bind.
+    intros l <- ms Hsplitm.
+    eapply pure_ret_mono. { apply Hsplitm. }
+    intros [l1 l2] (Hl1 & Hl2 & Hperm).
+    rewrite <- Hperm in Hpre; apply Forall_app in Hpre as [??].
     simpl_extend; simpl.
+
     eapply pure_eval_let.
-    { eapply pure_eval_app. pure_path. pure_path.
-      encode. (* FIXME *)
-      (* Use the induction hypothesis on [l1] *)
-      apply IH.
-      { (* Subgoal: show [length l1 < length l ] *)
-        rewrite Heql; rewrite Heql in Hl1. apply div2_lt_succ; auto. }
-      { (* Subgoal: show that [l1] ⊨ [mergesort_pre] *)
-        assumption. } }
+    { eapply (pure_EApp tele[list Z]).
+      eapply pure_eval_path. simpl. rewrite Hmergesort. pure_ret.
+      eapply pure_eval_path. eapply pure_ret. encode. apply eq_refl.
+      unfold arg_bind.
+      intros l -> mm Hcall.
+      apply Hcall.
+      - simpl in Hperm, Hl1, Hl2.
+        rewrite Heql in Hl1, Hl2 |-*.
+        apply div2_lt_succ. apply Hl1.
+      - assumption. }
+
     intros l1' IHl1'.
     eapply pure_eval_let.
-    { eapply pure_eval_app. pure_path. pure_path.
-      encode. (* FIXME *)
-      (* Use the induction hypothesis on [l2] *)
-      apply IH.
-      { (* Subgoal: show [length l2 < length l] *)
-        rewrite Hl2 Heql. auto with arith. }
-      { (* Subgoal: show that [l2] ⊨ [mergesort_pre] *)
-        assumption. } }
+    { eapply (pure_EApp tele[list Z]).
+      eapply pure_eval_path. simpl. rewrite Hmergesort. pure_ret.
+      eapply pure_eval_path. eapply pure_ret. encode. apply eq_refl.
+      unfold arg_bind.
+      intros ? -> mm Hcall. apply Hcall.
+      - rewrite Hl2. simpl. destruct (length x0); auto with arith.
+        inversion Heql. auto with arith.
+      - assumption. }
+
     intros l2' IHl2'; clear IH Hl1 Hl2 Heql m.
-    eapply pure_eval_app2_conseq.
-    { (* Use the knowledge that [merge] ∈ [η] *)
-      eapply pure_eval_path. simpl. rewrite Hmerge. pure_ret. }
-    { pure_path. encode. }
-    { pure_path. encode. }
-    (* Use the knowledge that [merge] ⊨ [_merge_spec] *)
-    { apply _merge_spec.
-      (* Show that [l1'], [l2'] ⊨ [merge_pre] *)
-      unfold mergesort_pre, mergesort_post in *.
-      destruct_hyps IHl1' IHl2'.
-      split; [ by rewrite_permutation l1'
-             | split;
-               [ by rewrite_permutation l2'
-               | auto ]
-        ]. }
-    intros l' IH.
-    (* Subgoal: show that [l'] ⊨ [mergesort_post] *)
-    unfold mergesort_post, merge_post in *.
-    destruct_hyps IHl1' IHl2' IH.
-    split; [ assumption | ].
-    rewrite_permutation l'. rewrite_permutation (x :: x0).
-    rewrite_permutation l1'. rewrite_permutation l2'.
-    reflexivity. }
+    abstract_env.
+    eapply (pure_EApp tele[list Z; list Z]).
+    - (* Use the knowledge that [merge] ∈ [η] *)
+      eapply pure_eval_path. simpl; rewrite Hmerge. pure_ret.
+    - eapply pure_eval_path. eapply pure_ret. encode. apply eq_refl.
+    - eapply pure_eval_path. eapply pure_ret. encode. apply eq_refl.
+    - simpl. intros ? ? <-. unfold arg_app. intros <- m Hmerge'.
+      unfold merge_spec in Hmerge'.
+      simpl in IHl1', IHl2'; destruct IHl1' as [??]; destruct IHl2' as [??].
+      eapply pure_ret_mono. apply Hmerge'.
+      * split; [ by rewrite_permutation l1' | assumption ].
+      * split; [ by rewrite_permutation l2' | assumption ].
+      * intros l' IH.
+        (* Subgoal: show that [l'] ⊨ [mergesort_post] *)
+        cbn in IH; destruct IH as [??].
+        split; [ assumption | ].
+        rewrite_permutation l'. rewrite_permutation (x :: x0).
+        rewrite_permutation l1'. rewrite_permutation l2'.
+        reflexivity. }
 Qed.
 
-(* We use the [toplevel] judgement to specify the module
-   created by the whole [merge.ml] file.
+End merge.
 
-   [env_has_pspecs] takes an association list of names and
-   specifications. It returns the conjunction of each specification
-   applied to the lookup of its corresponding name. *)
 
 Lemma Module__spec' :
-  toplevel __main
-    (env_has_pspecs [("merge", merge_spec);
-                     ("split", split_spec)
-                     (* ("merge_sort", mergesort_spec) *)]).
+  eval_module stdlib_env __main (λ _, True).
 Proof.
-    apply module_struct.
-  next_item.
-  (* Evaluate "merge" letrec *)
-  { apply Merge_spec'. }
-  intros [??] (merge & Hmerge & -> & ->).
-  next_item.
-  (* Evaluate "split" letrec *)
-  { apply Split_spec'. }
-  intros [??] (split & Hsplit & -> & ->).
-  next_item.
+  apply module_struct.
+  eapply (@structs_letrec tele[list Z; list Z]) with
+    (P := merge_spec). repeat constructor.
+  { apply wf_double_list_length. }
+  { unfold unfold_spec; simpl.
+
+    intros merge l1 l2 IH.
+    unfold merge_spec. intros [Hreprl1 Hsortl1] [Hreprl2 Hsortl2].
+    fold eval.
+    eapply pure_eval_match.
+    {
+      eapply pure_eval_pair.
+      eapply pure_eval_path. eapply pure_ret.
+      (* FIXME (IY): Automation for encode is broken. *)
+      rewrite encode_list_is_encode. encode.
+      pure_path.
+      (* FIXME: Automation for encode is broken. *)
+      rewrite encode_list_is_encode. encode. }
+    pure_match; abstract_env.
+
+    { pure_path. }
+    { pure_path. split; [ | rewrite app_nil_r ]; auto. }
+
+    eapply pure_eval_ifthenelse.
+    { (* Evaluate expression "h1 <= h2" *)
+      pure_EOpLe; repeat Forall_inversion; auto. }
+    { (* Evaluate expression "h1 :: (merge t1 l2)" knowing h1 <= h2 *)
+      intros.
+      eapply pure_eval_data. eapply pure_evals_cons.
+      pure_path.
+      (* FIXME (IY): Automation for encode is broken.
+         Probably encode shouldn't unfold here? *)
+      unfold observe, observe_encode. encode.
+      eapply @pure_evals_cons with (A := list Z).
+
+      (* Evaluate "merge t1 l2" under the cons *)
+      eapply (pure_EApp tele[list Z; list Z]).
+      { pure_path. }
+      { pure_path. apply eq_refl. }
+      { eapply pure_eval_path. eapply pure_ret.
+        encode. apply eq_refl. }
+      simpl; unfold arg_app.
+      intros t1 l2 -> Ht1.
+      intros m Hmerge.
+      unfold merge_spec in Hmerge.
+      all_inversions.
+      eapply pure_ret_mono.
+      { apply Hmerge.
+        - simpl; auto with arith. - split; auto. - split; auto. }
+      intros l [Hsorted Hpermutation].
+      eapply pure_evals_nil.
+      exists (x :: l).
+      split; [ encode | split ].
+      + (* Subgoal: the output is sorted *)
+        constructor; [ assumption | ].
+        eapply HdRel_Sorted_Permutation; eauto with zarith.
+      + (* Subgoal: the output is a permutation of the inputs *)
+        by rewrite_permutation l. }
+
+    { (* Evaluate expression "h2 :: (merge l1 t2)" knowing  (h1 > h2) *)
+      simpl; intros. fold eval.
+      eapply pure_eval_data. eapply pure_evals_cons.
+      pure_path.
+      (* FIXME *)
+      unfold observe, observe_encode. encode.
+      eapply @pure_evals_cons with (A := list Z).
+
+      (* Evaluate "merge l1 t2" under the cons *)
+      eapply (pure_EApp tele[list Z; list Z]).
+      { pure_path. }
+      { eapply pure_eval_path. eapply pure_ret. encode. apply eq_refl. }
+      { eapply pure_eval_path. eapply pure_ret. encode. apply eq_refl. }
+
+      unfold arg_bind, arg_app.
+      intros ? ? <- <-.
+      intros m Hmerge.
+      eapply pure_ret_mono.
+      { apply Hmerge.
+        - simpl; lia. - split; auto. - split; by all_inversions. }
+
+      intros l [Hsorted Hpermutation].
+      apply pure_evals_nil.
+      exists (x0 :: l).
+      split; [ encode | split ].
+      + (* Subgoal: the output is sorted *)
+        constructor; [ assumption | ].
+        eapply HdRel_Sorted_Permutation; eauto with zarith;
+          by all_inversions.
+      + (* Subgoal: the output is a permutation of the inputs *)
+        rewrite_permutation l.
+        apply Permutation_sym. apply Permutation_middle. } }
+
+  intros merge Hmerge.
+  eapply (structs_letrec tele[list Z]) with
+    (P := split_spec).
+  { apply list_wf. }
+  { intros split l IH. unfold split_spec.
+
+    eapply pure_eval_match. { pure_path. }
+    pure_match; abstract_env.
+
+    (* First branch of match *)
+    { (* Case: l matches [] *)
+      apply pure_eval_pair;
+        repeat (eapply pure_eval_const; encode).
+      (* Establish the (trivial) postcondition *)
+      split; simpl; auto. }
+    (* Second branch of match *)
+    { (* Case: l matches [x] *)
+      apply pure_eval_pair.
+      eapply pure_eval_data. eapply pure_evals_cons.
+      pure_path. simpl. encode.
+      eapply pure_evals_cons.
+      (* FIXME. *) eapply pure_eval_const with (x := @nil Z). encode.
+      eapply pure_evals_nil.
+      exists ([x]); split; [ encode | ].
+      eapply pure_eval_const. encode.
+      (* Establish postcondition *)
+      split; simpl; auto. }
+    (* Third branch of match *)
+    { (* Case: l matches a::b::t *)
+      eapply pure_eval_let_pair.
+      eapply (pure_EApp tele[list Z]).
+      { pure_path. }
+      { pure_path. apply eq_refl. }
+      unfold arg_bind.
+      intros l -> m Hsplit.
+      unfold split_spec in Hsplit.
+      eapply pure_ret_mono. { apply Hsplit. simpl; lia. }
+      intros [l1 l2] Hpost; clear IH; simpl.
+      (* FIXME. *)
+      simpl_extend; simpl. fold eval. abstract_env.
+      (* Eval (x1::l1, x2::l2) *)
+      apply pure_eval_pair.
+      eapply pure_eval_data. eapply pure_evals_cons. pure_path.
+      simpl; encode.
+      eapply pure_evals_cons. pure_path. simpl; encode.
+      eapply pure_evals_nil. exists (x1 :: l1); split; [ encode | ].
+      eapply pure_eval_data. eapply pure_evals_cons. pure_path.
+      simpl; encode.
+      eapply pure_evals_cons. pure_path. simpl; encode.
+      eapply pure_evals_nil. exists (x :: l2); split; [ encode | ].
+      (* Establish postcondition *)
+      unfold split_post in *; simpl in *.
+      subst.
+      destruct Hpost as (Hlength1 & Hlength2 & ?).
+      split; [ | split ].
+      { (* Subgoal: the length of l1 is half the length of xs *)
+        destruct (Nat.even _); rewrite Hlength1; eauto with arith. }
+      { (* Subgoal: the length of l2 is half the length of xs *)
+        rewrite Hlength2; eauto with arith. }
+      { (* Subgoal: l1++l2 is a permutation of xs *)
+        rewrite_permutation l.
+        apply Permutation_skip.
+        apply Permutation_sym.
+        apply Permutation_middle. } } }
+  intros split Hsplit.
+
   (* Evaluate "merge_sort" letrec *)
-  { apply MergeSort_spec; eauto. }
-  intros [??] (mergesort & Hmergesort & -> & ->).
+  eapply (@structs_letrec tele[list Z]) with
+    (P := mergesort_spec). repeat constructor.
+  { apply list_wf. }
+  { unfold unfold_spec; simpl.
+    intros mergesort l IH.
+    eapply mergesort_mkspec; eauto. }
+  intros mergesort Hmergesort.
   (* We have now evaluated the whole struct. *)
   finished_struct.
   (* Goal: Show that the resulting environment satisfies the spec. *)
